theories/Dot/examples/sem/syntyp_lemmas/sub_lr_syn.v
@@ -1,0 +1,27 @@
+(** * Semantic lemmas for double-delay subtyping. *)
+From iris.proofmode Require Import tactics.
+
+From D Require Import iris_prelude swap_later_impl.
+From D.Dot Require Import rules path_repl unary_lr dsub_lr defs_lr binding_lr sub_lr.
+
+Implicit Types (Σ : gFunctors)
+         (v w : vl) (e : tm) (d : dm) (ds : dms) (p : path)
+         (ρ : env) (l : label).
+
+Section defs.
+  Context {Σ}.
+
+  Definition istpi `{!dlangG Σ} Γ T1 T2 i j := sstpi i j V⟦Γ⟧* V⟦T1⟧ V⟦T2⟧.
+End defs.
+
+Notation "Γ ⊨ T1 , i <: T2 , j" := (istpi Γ T1 T2 i j) (at level 74, T1, T2, i, j at next level).
+
+Section judgment_lemmas.
+  Context `{!dlangG Σ}.
+
+  (** ** Show this typing judgment is equivalent to the more direct definition. *)
+  Lemma istpi_eq Γ T1 i T2 j :
+    Γ ⊨ T1, i <: T2, j ⊣⊢
+    |==> ∀ ρ v, G⟦Γ⟧ ρ → ▷^i V⟦T1⟧ anil ρ v → ▷^j V⟦T2⟧ anil ρ v.
+  Proof. reflexivity. Qed.
+End judgment_lemmas.
